src/QuerySemantic.v
@@ -3,58 +3,82 @@ Set Implicit Arguments.
 Unset Strict Implicit.
 Unset Printing Implicit Defensive.
 
+From extructures Require Import ord fmap.
 
 Require Import SchemaWellFormedness.
 Require Import Conformance.
 Require Import QueryConformance.
 Require Import SchemaAux.
+Require Import GraphAux.
 
+Require Import Schema.
 Require Import Query.
 Require Import Graph.
-Require Import Schema.
 
 
 
 Section QuerySemantic.
 
-  Variables N Name Vals : finType.
+  Variables N Name Vals : ordType.
 
-  Inductive eval (schema : @wfSchema Name Vals) (graph : @conformedGraph N Vals Name schema) : @Query Name Name Name Vals  -> @ResponseObject Name Vals  -> Prop :=
-  | EvField : forall (u : N) (f : fld) (value : Vals),
-      (λ graph) (u, f) = Some (inl value) ->
-      SelectionConforms schema (SingleField (label f) (args f)) ((τ graph) u) ->
-      eval graph (SingleField (label f) (args f)) (SingleResult (label f) value)
 
-  | EvNullField : forall (u : N) (f : fld),
-      (λ graph) (u, f) = None ->
-      eval graph (SingleField (label f) (args f)) (Null (label f))
+  Fixpoint eval (schema : @wfSchema Name Vals)  (g : graphQLGraph) (u : @node N Name Vals) (query : Query) : @ResponseObject Name Vals :=
+    match query with
+    | SingleField name args => match u.(fields) (Field name args) with
+                              | Some (inl value) => SingleResult name value
+                              | _ => Null name
+                              end
+    | LabeledField label name args =>  match u.(fields) (Field name args) with
+                                      | Some (inl value) => SingleResult label value
+                                      | _ => Null name
+                                      end
+    | NestedField name args ϕ => let target_nodes := get_target_nodes_with_field g u (Field name args) in
+                                match lookupFieldType schema u.(type) name with
+                                | Some (ListType _) =>
+                                  NestedListResult name (map (fun v => eval schema g v ϕ) target_nodes)
+                                | Some (NamedType _) =>
+                                  match ohead target_nodes with
+                                  | Some v => (NestedResult name (eval schema g v ϕ))
+                                  | _ => Null name
+                                  end
+                                | _ => Null name         (* If the field ∉ fields(u) then it's null, right? *)
+                                end
+                                    
+    | NestedLabeledField label name args ϕ =>  let target_nodes := get_target_nodes_with_field g u (Field name args) in
+                                match lookupFieldType schema u.(type) name with
+                                | Some (ListType _) =>
+                                  NestedListResult label (map (fun v => eval schema g v ϕ) target_nodes)
+                                | Some (NamedType _) =>
+                                  match ohead target_nodes with
+                                  | Some v => (NestedResult label (eval schema g v ϕ))
+                                  | _ => Null name
+                                  end
+                                | _ => Null name         
+                                end
+    | InlineFragment t ϕ => match lookupName schema t with
+                           | Some (ObjectTypeDefinition _ _ _) => if t == (NamedType u.(type)) then
+                                                                   eval schema g u ϕ
+                                                                 else
+                                                                   Empty
+                           | Some (InterfaceTypeDefinition _ _) => if declaresImplementation schema (NamedType u.(type)) t then
+                                                                    eval schema g u ϕ
+                                                                  else
+                                                                    Empty
+                           | Some (UnionTypeDefinition _ mbs) => if (NamedType u.(type)) \in mbs then
+                                                                  eval schema g u ϕ
+                                                                else
+                                                                  Empty
+                           | _ => Empty
+                           end
+    | SelectionSet ϕ ϕ' => ResponseList (eval schema g u ϕ) (eval schema g u ϕ')
+    end.
 
-  | EvLabeledField :  forall (u : N) (f : fld) (value : Vals) (l : Name),
-      (λ graph) (u, f) = Some (inl value) ->
-      SelectionConforms schema (LabeledField l (label f) (args f)) ((τ graph) u) ->
-      eval graph (LabeledField l (label f) (args f)) (SingleResult (label f) value)
 
-  | EvNullLabeledField :  forall (u : N) (f : fld) (l : Name),
-      (λ graph) (u, f) = None ->
-      eval graph (LabeledField l (label f) (args f)) (Null (label f))
-(*
-  | EvNestedListField :
+  Definition eval_query (schema : @wfSchema Name Vals)  (g : @conformedGraph N Name Vals schema) (query : @wfQuery Name Vals schema) : @ResponseObject Name Vals :=
+    let: WFQuery query _ := query in
+    eval schema g.(graph) g.(graph).(root) query.
 
-  | EvNestedField :
-
-  | EvNullNestedField :
-
-  | EvNestedLabeledListField :
-
-  | EvNestedLabeledField :
-
-  | EvNullNestedLabeledField : *)
-
-  | EvInlineFragment : forall (u : N) (t : Name) (ϕ : Query),
-      ((isObjectType schema (NamedType t)) && (((τ graph) u) == t)) ||
-       ((isInterfaceType schema (NamedType t)) && (declaresImplementation schema t ((τ graph) u)))  ->
-       eval graph (InlineFragment t ϕ) (Null t)
-    .
-
+    
+      
 
 End QuerySemantic.
